Adapt ProofData for new compilation

regex/Regex/NFA/Compile/ProofData/Basic.lean
@@ -2,7 +2,7 @@
 module
 
 public import Regex.NFA.Compile.Basic
-import all Regex.NFA.Compile.Basic
+-- import all Regex.NFA.Compile.Basic
 public import Regex.NFA.Compile.Lemmas
 
 open Regex.Data (Classes Expr)
@@ -21,6 +21,7 @@ namespace ProofData
 
 variable [ProofData]
 
+@[grind =]
 def nfa' : NFA := nfa.pushRegex next e
 
 theorem size_lt : nfa.size < nfa'.size := pushRegex_size_lt
@@ -40,39 +41,40 @@ class Empty extends ProofData where
 
 namespace Empty
 
+@[grind =]
 def intro {nfa next result} (_ : NFA.pushRegex nfa next .empty = result) : Empty :=
   { nfa, next, e := .empty, expr_eq := rfl }
 
+@[grind =]
 def intro' (nfa : NFA) (next : Nat) : Empty :=
   { nfa, next, e := .empty, expr_eq := rfl }
 
 variable [Empty]
 
+@[grind =]
 theorem eq' : nfa' = nfa.pushRegex next .empty := by
   simp [nfa', expr_eq]
 
+@[grind =]
 theorem start_eq : nfa'.start = nfa.size := by
   simp [eq', pushRegex]
 
+@[grind =]
 theorem size_eq : nfa'.size = nfa.size + 1 := by
   simp [eq', pushRegex]
 
+@[grind =]
 theorem get_lt {i : Nat} (h : i < nfa.size) : nfa'[i]'(Nat.lt_trans h size_lt) = nfa[i] := by
   simp [eq', pushRegex, pushNode_get_lt i h]
 
+@[grind =]
 theorem get_eq : nfa'[nfa.size]'size_lt = .fail := by
   simp [eq', pushRegex]
 
+@[grind =]
 theorem get (i : Nat) (h : i < nfa'.size) :
-  if _ : i < nfa.size then nfa'[i] = nfa[i]
-  else nfa'[i] = .fail := by
-  split
-  case isTrue => exact get_lt _
-  case isFalse h' =>
-    have : i = nfa.size := by
-      simp [size_eq] at h
-      omega
-    simp [this, get_eq]
+  nfa'[i] = if _ : i < nfa.size then nfa[i] else .fail := by
+  grind
 
 end Empty
 
@@ -81,39 +83,40 @@ class Epsilon extends ProofData where
 
 namespace Epsilon
 
+@[grind =]
 def intro {nfa next result} (_ : NFA.pushRegex nfa next .epsilon = result) : Epsilon :=
   { nfa, next, e := .epsilon, expr_eq := rfl }
 
+@[grind =]
 def intro' (nfa : NFA) (next : Nat) : Epsilon :=
   { nfa, next, e := .epsilon, expr_eq := rfl }
 
 variable [Epsilon]
 
+@[grind =]
 theorem eq' : nfa' = nfa.pushRegex next .epsilon := by
   simp [nfa', expr_eq]
 
+@[grind =]
 theorem start_eq : nfa'.start = nfa.size := by
   simp [eq', pushRegex]
 
+@[grind =]
 theorem size_eq : nfa'.size = nfa.size + 1 := by
   simp [eq', pushRegex]
 
+@[grind =]
 theorem get_lt {i : Nat} (h : i < nfa.size) : nfa'[i]'(Nat.lt_trans h size_lt) = nfa[i] := by
   simp [eq', pushRegex, pushNode_get_lt i h]
 
+@[grind =]
 theorem get_eq : nfa'[nfa.size]'size_lt = .epsilon next := by
   simp [eq', pushRegex]
 
+@[grind =]
 theorem get (i : Nat) (h : i < nfa'.size) :
-  if _ : i < nfa.size then nfa'[i] = nfa[i]
-  else nfa'[i] = .epsilon next := by
-  split
-  case isTrue => exact get_lt _
-  case isFalse h' =>
-    have : i = nfa.size := by
-      simp [size_eq] at h
-      omega
-    simp [this, get_eq]
+  nfa'[i] = if _ : i < nfa.size then nfa[i] else .epsilon next := by
+  grind
 
 end Epsilon
 
@@ -123,39 +126,40 @@ class Anchor extends ProofData where
 
 namespace Anchor
 
+@[grind =]
 def intro {nfa next anchor result} (_ : NFA.pushRegex nfa next (.anchor anchor) = result) : Anchor :=
   { nfa, next, e := .anchor anchor, anchor, expr_eq := rfl }
 
+@[grind =]
 def intro' (nfa : NFA) (next : Nat) (anchor : Data.Anchor) : Anchor :=
   { nfa, next, e := .anchor anchor, anchor, expr_eq := rfl }
 
 variable [Anchor]
 
+@[grind =]
 theorem eq' : nfa' = nfa.pushRegex next (.anchor anchor) := by
   simp [nfa', expr_eq]
 
+@[grind =]
 theorem start_eq : nfa'.start = nfa.size := by
   simp [eq', pushRegex]
 
+@[grind =]
 theorem size_eq : nfa'.size = nfa.size + 1 := by
   simp [eq', pushRegex]
 
+@[grind =]
 theorem get_lt {i : Nat} (h : i < nfa.size) : nfa'[i]'(Nat.lt_trans h size_lt) = nfa[i] := by
   simp [eq', pushRegex, pushNode_get_lt i h]
 
+@[grind =]
 theorem get_eq : nfa'[nfa.size]'size_lt = .anchor anchor next := by
   simp [eq', pushRegex]
 
+@[grind =]
 theorem get (i : Nat) (h : i < nfa'.size) :
-  if _ : i < nfa.size then nfa'[i] = nfa[i]
-  else nfa'[i] = .anchor anchor next := by
-  split
-  case isTrue => exact get_lt _
-  case isFalse h' =>
-    have : i = nfa.size := by
-      simp [size_eq] at h
-      omega
-    simp [this, get_eq]
+  nfa'[i] = if _ : i < nfa.size then nfa[i] else .anchor anchor next := by
+  grind
 
 end Anchor
 
@@ -165,39 +169,40 @@ class Char extends ProofData where
 
 namespace Char
 
+@[grind =]
 def intro {nfa next c result} (_ : NFA.pushRegex nfa next (.char c) = result) : Char :=
   { nfa, next, e := .char c, c, expr_eq := rfl }
 
+@[grind =]
 def intro' (nfa : NFA) (next : Nat) (c : _root_.Char) : Char :=
   { nfa, next, e := .char c, c, expr_eq := rfl }
 
 variable [Char]
 
+@[grind =]
 theorem eq' : nfa' = nfa.pushRegex next (.char c) := by
   simp [nfa', expr_eq]
 
+@[grind =]
 theorem start_eq : nfa'.start = nfa.size := by
   simp [eq', pushRegex]
 
+@[grind =]
 theorem size_eq : nfa'.size = nfa.size + 1 := by
   simp [eq', pushRegex]
 
+@[grind =]
 theorem get_lt {i : Nat} (h : i < nfa.size) : nfa'[i]'(Nat.lt_trans h size_lt) = nfa[i] := by
   simp [eq', pushRegex, pushNode_get_lt i h]
 
+@[grind =]
 theorem get_eq : nfa'[nfa.size]'size_lt = .char c next := by
   simp [eq', pushRegex]
 
+@[grind =]
 theorem get (i : Nat) (h : i < nfa'.size) :
-  if _ : i < nfa.size then nfa'[i] = nfa[i]
-  else nfa'[i] = .char c next := by
-  split
-  case isTrue => exact get_lt _
-  case isFalse h' =>
-    have : i = nfa.size := by
-      simp [size_eq] at h
-      omega
-    simp [this, get_eq]
+  nfa'[i] = if _ : i < nfa.size then nfa[i] else .char c next := by
+  grind
 
 end Char
 
@@ -207,39 +212,40 @@ class Classes extends ProofData where
 
 namespace Classes
 
+@[grind =]
 def intro {nfa next cs result} (_ : NFA.pushRegex nfa next (.classes cs) = result) : Classes :=
   { nfa, next, e := .classes cs, cs, expr_eq := rfl }
 
+@[grind =]
 def intro' (nfa : NFA) (next : Nat) (cs : Data.Classes) : Classes :=
   { nfa, next, e := .classes cs, cs, expr_eq := rfl }
 
 variable [Classes]
 
+@[grind =]
 theorem eq' : nfa' = nfa.pushRegex next (.classes cs) := by
   simp [nfa', expr_eq]
 
+@[grind =]
 theorem start_eq : nfa'.start = nfa.size := by
   simp [eq', pushRegex]
 
+@[grind =]
 theorem size_eq : nfa'.size = nfa.size + 1 := by
   simp [eq', pushRegex]
 
+@[grind =]
 theorem get_lt {i : Nat} (h : i < nfa.size) : nfa'[i]'(Nat.lt_trans h size_lt) = nfa[i] := by
   simp [eq', pushRegex, pushNode_get_lt i h]
 
+@[grind =]
 theorem get_eq : nfa'[nfa.size]'size_lt = .sparse cs next := by
   simp [eq', pushRegex]
 
+@[grind =]
 theorem get (i : Nat) (h : i < nfa'.size) :
-  if _ : i < nfa.size then nfa'[i] = nfa[i]
-  else nfa'[i] = .sparse cs next := by
-  split
-  case isTrue => exact get_lt _
-  case isFalse h' =>
-    have : i = nfa.size := by
-      simp [size_eq] at h
-      omega
-    simp [this, get_eq]
+  nfa'[i] = if _ : i < nfa.size then nfa[i] else .sparse cs next := by
+  grind
 
 end Classes
 
@@ -250,15 +256,20 @@ class Group extends ProofData where
 
 namespace Group
 
+@[grind =]
 def intro {nfa next tag e' result} (_ : NFA.pushRegex nfa next (.group tag e') = result) : Group :=
   { nfa, next, e := .group tag e', tag, e', expr_eq := rfl }
 
+@[grind =]
 def intro' (nfa : NFA) (next : Nat) (tag : Nat) (e' : Expr) : Group :=
   { nfa, next, e := .group tag e', tag, e', expr_eq := rfl }
 
 variable [Group]
 
+@[grind =]
 def nfaClose : NFA := nfa.pushNode (.save (2 * tag + 1) next)
+
+@[grind =]
 def nfaExpr : NFA := nfaClose.pushRegex nfaClose.start e'
 
 theorem nfaClose_property : nfa.size < nfaClose.size := by simp [nfaClose]
@@ -266,11 +277,20 @@ theorem nfaClose_property : nfa.size < nfaClose.size := by simp [nfaClose]
 theorem nfaExpr_property : nfaClose.size < nfaExpr.size :=
   pushRegex_size_lt
 
+theorem wfClose (wf : nfa.WellFormed) (next_lt : next < nfa.size) : nfaClose.WellFormed := by
+  grind
+
+theorem wfExpr (wf : nfa.WellFormed) (next_lt : next < nfa.size) : nfaExpr.WellFormed := by
+  grind
+
+@[grind =]
 theorem eq' : nfa' = nfa.pushRegex next (.group tag e') := by
   simp [nfa', expr_eq]
 
+@[grind =]
 theorem eq_push : nfa' = nfaExpr.pushNode (.save (2 * tag) nfaExpr.start) := eq'
 
+@[grind =]
 theorem start_eq : nfa'.start = nfaExpr.size := by
   simp [eq_push]
 
@@ -283,16 +303,14 @@ theorem size_lt_close' : nfaClose.size < nfa'.size :=
 theorem size_lt_nfa_expr : nfa.size < nfaExpr.size :=
   Nat.lt_trans nfaClose_property nfaExpr_property
 
-theorem get_open : nfa'[nfaExpr.size]'size_lt_expr' = (.save (2 * tag) nfaExpr.start) := by
-  simp [eq_push]
-
-theorem get_lt_expr {i : Nat} (h : i < nfaExpr.size) :
-  nfa'[i]'(Nat.lt_trans h size_lt_expr') = nfaExpr[i] := by
-  simp [eq_push, pushNode_get_lt i h]
-
--- We state this for `nfaClose` for now because an inducion hypothesis is needed to see through `nfaExpr`.
-theorem get_close_pre : nfaClose[nfa.size]'nfaClose_property = .save (2 * tag + 1) next := by
-  simp [nfaClose]
+@[grind =]
+theorem get (i : Nat) (h : i < nfa'.size) :
+  nfa'[i] =
+    if _ : i < nfa.size then nfa[i]
+    else if i = nfa.size then .save (2 * tag + 1) next
+    else if _ : i < nfaExpr.size then nfaExpr[i]
+    else .save (2 * tag) nfaExpr.start := by
+  grind
 
 end Group
 
@@ -303,15 +321,20 @@ class Alternate extends ProofData where
 
 namespace Alternate
 
+@[grind =]
 def intro {nfa next e₁ e₂ result} (_ : NFA.pushRegex nfa next (.alternate e₁ e₂) = result) : Alternate :=
   { nfa, next, e := .alternate e₁ e₂, e₁, e₂, expr_eq := rfl }
 
+@[grind =]
 def intro' (nfa : NFA) (next : Nat) (e₁ e₂ : Expr) : Alternate :=
   { nfa, next, e := .alternate e₁ e₂, e₁, e₂, expr_eq := rfl }
 
 variable [Alternate]
 
+@[grind =]
 def nfa₁ : NFA := nfa.pushRegex next e₁
+
+@[grind =]
 def nfa₂ : NFA := nfa₁.pushRegex next e₂
 
 theorem nfa₁_property : nfa.size < nfa₁.size :=
@@ -320,9 +343,17 @@ theorem nfa₁_property : nfa.size < nfa₁.size :=
 theorem nfa₂_property : nfa₁.size < nfa₂.size :=
   pushRegex_size_lt
 
+theorem wf₁ (wf : nfa.WellFormed) (next_lt : next < nfa.size) : nfa₁.WellFormed := by
+  grind
+
+theorem wf₂ (wf : nfa₁.WellFormed) (next_lt : next < nfa₁.size) : nfa₂.WellFormed := by
+  grind
+
+@[grind =]
 theorem eq' : nfa' = nfa.pushRegex next (.alternate e₁ e₂) := by
   simp [nfa', expr_eq]
 
+@[grind =]
 theorem eq_push : nfa' = nfa₂.pushNode (.split nfa₁.start nfa₂.start) := eq'
 
 theorem size_lt₂ : nfa₂.size < nfa'.size := by
@@ -331,14 +362,14 @@ theorem size_lt₂ : nfa₂.size < nfa'.size := by
 theorem size_lt₁ : nfa₁.size < nfa'.size :=
   Nat.lt_trans nfa₂_property size_lt₂
 
-theorem get_split : nfa'[nfa₂.size]'size_lt₂ = .split nfa₁.start nfa₂.start := by
-  simp [eq_push]
-
-theorem start_eq : nfa'.start = nfa₂.size := by
-  simp [eq_push]
-
-theorem get_start : nfa'[nfa'.start]'(start_eq ▸ size_lt₂) = .split nfa₁.start nfa₂.start := by
-  simp [start_eq, get_split]
+@[grind =]
+theorem get (i : Nat) (h : i < nfa'.size) :
+  nfa'[i] =
+    if _ : i < nfa.size then nfa[i]
+    else if _ : i < nfa₁.size then nfa₁[i]
+    else if _ : i < nfa₂.size then nfa₂[i]
+    else .split nfa₁.start nfa₂.start := by
+  grind
 
 end Alternate
 
@@ -349,22 +380,30 @@ class Concat extends ProofData where
 
 namespace Concat
 
+@[grind =]
 def intro {nfa next e₁ e₂ result} (_ : NFA.pushRegex nfa next (.concat e₁ e₂) = result) : Concat :=
   { nfa, next, e := .concat e₁ e₂, e₁, e₂, expr_eq := rfl }
 
+@[grind =]
 def intro' (nfa : NFA) (next : Nat) (e₁ e₂ : Expr) : Concat :=
   { nfa, next, e := .concat e₁ e₂, e₁, e₂, expr_eq := rfl }
 
 variable [Concat]
 
+@[grind =]
 def nfa₂ : NFA := nfa.pushRegex next e₂
 
 theorem nfa₂_property : nfa.size < nfa₂.size :=
   pushRegex_size_lt
 
+theorem wf₂ (wf : nfa.WellFormed) (next_lt : next < nfa.size) : nfa₂.WellFormed := by
+  grind
+
+@[grind =]
 theorem eq' : nfa' = nfa.pushRegex next (.concat e₁ e₂) := by
   simp [nfa', expr_eq]
 
+@[grind =]
 theorem eq_push : nfa' = nfa₂.pushRegex nfa₂.start e₁ := by
   simp [eq', pushRegex]
   rfl
@@ -372,6 +411,14 @@ theorem eq_push : nfa' = nfa₂.pushRegex nfa₂.start e₁ := by
 theorem size₂_lt : nfa₂.size < nfa'.size := by
   simp [eq_push]
   exact pushRegex_size_lt
+
+@[grind =]
+theorem get (i : Nat) (h : i < nfa'.size) :
+  nfa'[i] =
+    if _ : i < nfa.size then nfa[i]
+    else if _ : i < nfa₂.size then nfa₂[i]
+    else (nfa₂.pushRegex nfa₂.start e₁)[i]'(by grind) := by
+  grind
 
 end Concat
 
@@ -382,19 +429,38 @@ class Star extends ProofData where
 
 namespace Star
 
+@[grind =]
 def intro {nfa next greedy e' result} (_ : NFA.pushRegex nfa next (.star greedy e') = result) : Star :=
   { nfa, next, e := .star greedy e', greedy, e', expr_eq := rfl }
 
+@[grind =]
 def intro' (nfa : NFA) (next : Nat) (greedy : Bool) (e': Expr) : Star :=
   { nfa, next, e := .star greedy e', greedy, e', expr_eq := rfl }
 
 variable [Star]
 
+@[grind =]
 theorem eq' : nfa' = nfa.pushRegex next (.star greedy e') := by
   simp [nfa', expr_eq]
 
+@[grind =]
 def nfaPlaceholder : NFA := nfa.pushNode .fail
-def nfaExpr : NFA := nfaPlaceholder.pushRegex nfaPlaceholder.start e'
+
+@[grind =]
+def nfaExpr : NFA := nfaPlaceholder.pushRegex nfa.size e'
+
+@[grind =]
+def split : Node := if greedy then .split nfaExpr.start next else .split next nfaExpr.start
+
+@[grind =]
+def quest : NFA := nfaExpr.pushNode split
+
+@[grind =]
+def patched : NFA := ⟨quest.nodes.setIfInBounds nfa.size split⟩
+
+@[grind =]
+theorem eq_patched : nfa' = patched := by
+  grind
 
 theorem nfaPlaceholder_property : nfa.size < nfaPlaceholder.size := by
   simp [nfaPlaceholder]
@@ -402,25 +468,46 @@ theorem nfaPlaceholder_property : nfa.size < nfaPlaceholder.size := by
 theorem nfaExpr_property : nfaPlaceholder.size < nfaExpr.size :=
   pushRegex_size_lt
 
-theorem start_eq : nfa'.start = nfa.size := by
-  rw [eq', pushRegex]
+theorem size_eq_patched : nfa'.size = patched.size := by
+  grind
 
-theorem size_eq_expr' : nfa'.size = nfaExpr.size := by
-  simp only [expr_eq, pushRegex, nfa', nfaExpr, nfaPlaceholder, pushNode_start_eq, size]
-  rw [Array.size_setIfInBounds]
+theorem size_eq_quest : nfa'.size = quest.size := by
+  grind
 
-def splitNode : NFA.Node :=
-  .split (if greedy then nfaExpr.start else next) (if greedy then next else nfaExpr.start)
+theorem wfPlaceholder (wf : nfa.WellFormed) : nfaPlaceholder.WellFormed := by
+  grind
 
-theorem get_start : nfa'[nfa.size]'size_lt = splitNode := by
-  simp [eq', pushRegex, NFA.get_eq_nodes_get, splitNode]
-  split <;> rfl
+theorem wfExpr (wf : nfa.WellFormed) : nfaExpr.WellFormed := by
+  grind
 
-theorem get_ne_start (i : Nat) (h : i < nfa'.size) (ne : i ≠ nfa.size) :
-  nfa'[i] = nfaExpr[i]'(size_eq_expr' ▸ h) := by
-  simp [eq', pushRegex, NFA.get_eq_nodes_get, nfaExpr]
-  have hj : i < nfaExpr.nodes.size := (by rfl : nfaExpr.size = nfaExpr.nodes.size) ▸ (size_eq_expr' ▸ h)
-  exact Array.getElem_setIfInBounds_ne (hj := hj) (h := ne.symm)
+theorem wfQuest (wf : nfa.WellFormed) (next_lt : next < nfa.size) : quest.WellFormed := by
+  grind
+
+theorem wfPatched (wf : nfa.WellFormed) (next_lt : next < nfa.size) : patched.WellFormed :=
+  eq_patched ▸ pushRegex_wf wf next_lt
+
+@[grind =]
+theorem start_eq : nfa'.start = nfaExpr.size := by
+  simp [start, size_eq_quest, quest]
+
+@[grind =]
+theorem get (i : Nat) (h : i < nfa'.size) :
+  nfa'[i] =
+    if _ : i < nfa.size then nfa[i]
+    else if i = nfa.size then split
+    else if _ : i < nfaExpr.size then nfaExpr[i]
+    else split := by
+  if h' : i < nfa.size then
+    grind
+  else if h' : i = nfa.size then
+    grind
+  else
+    conv =>
+      lhs
+      simp only [eq_patched, patched, get_eq_nodes_get,
+        Array.getElem_setIfInBounds_ne (show i < quest.size by grind) (show nfa.size ≠ i by grind)]
+      rw [← get_eq_nodes_get]
+    grind
 
 end Star
 
