regex/Regex/NFA/Compile.lean
@@ -2,4 +2,4 @@ module
 
 public import Regex.NFA.Compile.Basic
 public import Regex.NFA.Compile.Lemmas
--- public import Regex.NFA.Compile.ProofData
+public import Regex.NFA.Compile.ProofData
