regex/Regex/NFA/Compile/ProofData.lean
@@ -1,4 +1,3 @@
 module
 
 public import Regex.NFA.Compile.ProofData.Basic
-public import Regex.NFA.Compile.ProofData.Lemmas
